Progress towards factoring backend/proofs
In particular create a word_gcFunctions theory to house a bunch of
definitions and minor theorems used by a number of ...Proof scripts.
Rather than have these in one of the Proof files, moving them into
their own separate file lets the Proof files run concurrently and
doesn't misrepresent the conceptual dependency story.

compiler/backend/proofs/stack_removeProofScript.sml
@@ -2087,9 +2087,6 @@ val star_move_lemma = Q.prove(
   `p0 * p1 * p2 * p3 * p4 = p2 * (p1 * STAR p3 (p4 * p0))`,
   fs [AC STAR_COMM STAR_ASSOC]);
 
-(* TODO: let's not repeat these everywhere *)
-val isWord_def = Define `(isWord (Word w) = T) /\ (isWord _ = F)`
-val theWord_def = Define `theWord (Word w) = w`
 
 val read_mem_def = Define `
   (read_mem a m 0 = []) /\
@@ -2500,13 +2497,14 @@ val init_code_thm = Q.store_thm("init_code_thm",
     \\ rfs [] \\ decide_tac) \\ strip_tac
   \\ qunabbrev_tac `s8`
   \\ qunabbrev_tac `s7`
-  \\ fs [FUPDATE_LIST,FAPPLY_FUPDATE_THM,theWord_def,FLOOKUP_UPDATE,mem_val_def]
+  \\ fs [FUPDATE_LIST,FAPPLY_FUPDATE_THM,wordSemTheory.theWord_def,
+         FLOOKUP_UPDATE,mem_val_def]
   \\ fs [store_init_def,store_list_def,UPDATE_LIST_def,APPLY_UPDATE_THM,
          FLOOKUP_UPDATE,word_store_def,mem_val_def,FAPPLY_FUPDATE_THM]
   \\ fs [FLOOKUP_DEF,GSYM word_add_n2w,WORD_LEFT_ADD_DISTRIB]
   \\ fs [ONCE_REWRITE_RULE [MULT_COMM] MULT_DIV,LENGTH_read_mem,
-         theWord_def,init_prop_def,the_SOME_Word_def,is_SOME_Word_def,
-         FLOOKUP_UPDATE]
+         wordSemTheory.theWord_def,init_prop_def,the_SOME_Word_def,
+         is_SOME_Word_def, FLOOKUP_UPDATE]
   \\ fs [GSYM CONJ_ASSOC]
   \\ `read_mem (n2w (d * h2)) m1 (LENGTH heap) = heap` by
    (match_mp_tac(GEN_ALL(ONCE_REWRITE_RULE[STAR_COMM]word_list_IMP_read_mem))
